examples/LeakyLog.lean
@@ -1,0 +1,28 @@
+import JSCore.Syntax
+import JSCore.Values
+import JSCore.Eval
+import JSCore.Trace
+import JSCore.Properties
+import JSCore.Taint
+import JSCore.Tactics
+
+open JSCore
+
+def leakyLog_body : Expr :=
+  (.call "unsafeHash.digest"
+    [("arg0", (.var "secret"))]
+    "tag"
+    (.letConst "logLine"
+      (.binOp .add
+        (.binOp .add
+          (.var "userId")
+          (.strLit ":"))
+        (.var "tag"))
+      (.call "logger.info"
+        [("arg0", (.var "logLine"))]
+        "__void_0"
+        Expr.none)))
+
+theorem leakyLog_secret_leaks_to_logs
+    : notTaintedIn leakyLog_body "secret" "logger.*" ["crypto.hmac"] = false := by
+  native_decide
